\[
\begin{aligned}
   \Border{}{a} 
&= \epsilon\\
   \Border{}{a \cdot c} 
&= \Border{}{\Border{}{a} \cdot c}
\end{aligned}
\]
because \(\Border{}{a} \cdot c = \epsilon \cdot c = c
\not\preccurlyeq a\). Thus
\[
  \Border{}{ac} = \Border{}{c} = \epsilon
\]
Now:
\[
 \Border{}{ac \cdot a} = \Border{}{ac} \cdot a
\]
since \(\Border{}{ac} \cdot a = \epsilon \cdot a = a
\preccurlyeq ac\). Hence
\[
  \Border{}{aca} = a
\]
Now:
\[
  \Border{}{aca \cdot b} = \Border{}{\Border{}{aca} \cdot b}
\]
because \(\Border{}{aca} \cdot b = ab \not\preccurlyeq
aca\). Therefore
\[
  \Border{}{acab} = \Border{}{ab}
\]
We have to compute \(\Border{}{ab}\):
\[
  \Border{}{a \cdot b} = \Border{}{\Border{}{a} \cdot b}
\]
since \(\Border{}{a} \cdot b = \epsilon \cdot b = b
\not\preccurlyeq a\). Thus
\begin{align*}
   \Border{}{acab}
&= \Border{}{ab}\\
&= \Border{}{b}\\ 
&= \epsilon
\end{align*}
Now
\[
  \Border{}{acab \cdot b} = \Border{}{\Border{}{acab} \cdot b}
\]
because \(\Border{}{acab} \cdot b = \epsilon \cdot b = b
\not\preccurlyeq acab\). Then
\[
  \Border{}{acabb} = \Border{}{b} = \epsilon
\]
Now
\[
  \Border{}{acabb \cdot a} = \Border{}{acabb} \cdot a
\]
since \(\Border{}{acabb} \cdot a = \epsilon \cdot a = a
\preccurlyeq acabb\). Therefore
\[
  \Border{}{acabba} = a
\]
Now
\[
  \Border{}{acabba \cdot c} = \Border{}{acabba} \cdot c
\]
because \(\Border{}{acabba} \cdot c = a \cdot c = ac
\preccurlyeq acabba\). Thus
\[
  \Border{}{acabbac} = ac
\]
Now
\[
  \Border{}{acabbac \cdot a} = \Border{}{acabbac} \cdot a
\]
since \(\Border{}{acabbac} \cdot a = ac \cdot a = aca
\preccurlyeq acabbac\). Hence
\[
  \Border{}{acabbaca} = aca
\]
Now
\[
  \Border{}{acabbaca \cdot b} = \Border{}{acabbaca} \cdot b
\]
because \(\Border{}{acabbaca} \cdot b = aca \cdot b = acab
\preccurlyeq acabbaca\). Then
\[
  \Border{}{acabbacab} = acab
\]
Finally
\[
  \Border{}{acabbacab \cdot b} = 
\]
since \(\Border{}{acabbacab} \cdot b = acab \cdot b = acabb
\preccurlyeq acabbacab\). Thus
\[
  \Border{}{acabbacabb} = acabb
\]
